Code review.

theories/VLSM/Core/VLSMProjections/VLSMTotalProjection.v
@@ -563,25 +563,30 @@ Definition VLSM_projection_finite_trace_project_app
 
 Definition VLSM_projection_finite_trace_project_app_rev
   : forall l l1' l2', VLSM_projection_finite_trace_project Hsimul l = l1' ++ l2' ->
-    exists l1 l2, l = l1 ++ l2 /\
+    exists l1 l2,
+      l = l1 ++ l2 /\
       VLSM_projection_finite_trace_project Hsimul l1 = l1' /\
       VLSM_projection_finite_trace_project Hsimul l2 = l2'
   := pre_VLSM_projection_finite_trace_project_app_rev _ _ label_project state_project.
 
 Definition VLSM_projection_finite_trace_project_in
-  : forall itemX itemY, pre_VLSM_projection_transition_item_project _ _ label_project state_project itemX = Some itemY ->
-    forall trX, In itemX trX -> In itemY (VLSM_projection_finite_trace_project Hsimul trX)
+  : forall itemX itemY,
+      pre_VLSM_projection_transition_item_project _ _ label_project state_project itemX = Some itemY ->
+    forall trX,
+      In itemX trX -> In itemY (VLSM_projection_finite_trace_project Hsimul trX)
   := pre_VLSM_projection_finite_trace_project_in _ _ label_project state_project.
 
 Definition VLSM_projection_finite_trace_last
   : forall sX trX,
-    finite_valid_trace_from X sX trX ->
-    state_project (finite_trace_last sX trX) = finite_trace_last (state_project sX) (VLSM_projection_finite_trace_project Hsimul trX)
+      finite_valid_trace_from X sX trX ->
+      state_project (finite_trace_last sX trX) = finite_trace_last (state_project sX)
+        (VLSM_projection_finite_trace_project Hsimul trX)
   := final_state_project _ _ _ _ Hsimul.
 
 Definition VLSM_projection_finite_valid_trace
   : forall sX trX,
-    finite_valid_trace X sX trX -> finite_valid_trace Y (state_project sX) (VLSM_projection_finite_trace_project Hsimul trX)
+      finite_valid_trace X sX trX -> finite_valid_trace Y (state_project sX)
+        (VLSM_projection_finite_trace_project Hsimul trX)
   := trace_project_preserves_valid_trace _ _ _ _ Hsimul.
 
 (** Any [VLSM_projection] determines a [VLSM_partial_projection], allowing us
@@ -599,7 +604,8 @@ Qed.
 
 Lemma VLSM_projection_finite_valid_trace_from
   : forall sX trX,
-    finite_valid_trace_from X sX trX -> finite_valid_trace_from Y (state_project sX) (VLSM_projection_finite_trace_project Hsimul trX).
+      finite_valid_trace_from X sX trX ->
+      finite_valid_trace_from Y (state_project sX) (VLSM_projection_finite_trace_project Hsimul trX).
 Proof.
   specialize VLSM_partial_projection_from_projection as Hpart_simul.
   specialize (VLSM_partial_projection_finite_valid_trace_from Hpart_simul) as Hivt.
@@ -629,7 +635,9 @@ Definition VLSM_projection_input_valid
 
 Definition VLSM_projection_finite_valid_trace_from_to
   : forall sX s'X trX,
-    finite_valid_trace_from_to X sX s'X trX -> finite_valid_trace_from_to Y (state_project sX) (state_project s'X) (VLSM_projection_finite_trace_project Hsimul trX)
+      finite_valid_trace_from_to X sX s'X trX ->
+      finite_valid_trace_from_to Y (state_project sX) (state_project s'X)
+        (VLSM_projection_finite_trace_project Hsimul trX)
   := VLSM_weak_projection_finite_valid_trace_from_to VLSM_projection_weaken.
 
 Definition VLSM_projection_in_futures
@@ -659,7 +667,9 @@ Qed.
 
 Lemma VLSM_projection_finite_valid_trace_init_to
   : forall sX s'X trX,
-    finite_valid_trace_init_to X sX s'X trX -> finite_valid_trace_init_to Y (state_project sX) (state_project s'X) (VLSM_projection_finite_trace_project Hsimul trX).
+      finite_valid_trace_init_to X sX s'X trX ->
+      finite_valid_trace_init_to Y (state_project sX) (state_project s'X)
+        (VLSM_projection_finite_trace_project Hsimul trX).
 Proof.
   intros. destruct H as [H Hinit]. split.
   - revert H. apply VLSM_projection_finite_valid_trace_from_to.
@@ -722,7 +732,7 @@ Proof.
   apply valid_trace_forget_last in Htr.
   apply Hfr in Htr as [isX [trX [Htr [His Htr_pr]]]].
   apply VLSM_projection_finite_trace_project_app_rev in Htr_pr
-    as [trX_s1 [trX_s2 [HeqtrX [Htr_s1_pr Htr_s2_pr]]]].
+    as (trX_s1 & trX_s2 & HeqtrX & Htr_s1_pr & Htr_s2_pr).
   subst.
   destruct Htr as [HtrX HisX].
   apply finite_valid_trace_from_app_iff in HtrX as HtrX12.
